finished 2 exercises in Imp.v

Imp.v
@@ -793,13 +793,11 @@ Proof.
     + rewrite IHbevalR. reflexivity.
     + rewrite IHbevalR1. rewrite IHbevalR2. reflexivity.
   - generalize dependent bv.
-    induction b; intros; subst.
-    + apply E_BTrue.
-    + apply E_BFalse.
-    + apply E_BEq; rewrite aeval_iff_aevalR; reflexivity.
-    + apply E_BLe; rewrite aeval_iff_aevalR; reflexivity.
-    + apply E_BNot. apply IHb. reflexivity.
-    + apply E_BAnd. apply IHb1. reflexivity. apply IHb2. reflexivity.
+    induction b; intros; subst; constructor; repeat rewrite aeval_iff_aevalR; 
+    try reflexivity.
+    + apply IHb. reflexivity.
+    + apply IHb1. reflexivity. 
+    + apply IHb2. reflexivity.
 Qed.
 End AExp.
 
@@ -1366,8 +1364,10 @@ Example ceval_example2:
   (X ::= 0;; Y ::= 1;; Z ::= 2) / { --> 0 } \\
   { X --> 0 ; Y --> 1 ; Z --> 2 }.
 Proof.
-  (* FILL IN HERE *) Admitted.
-(** [] *)
+  apply E_Seq with { X --> 0 }.
+  - apply E_Ass. reflexivity.
+  - apply E_Seq with { X --> 0; Y --> 1 }. apply E_Ass; reflexivity.
+Qed.
 
 (** **** Exercise: 3 stars, optional (pup_to_n)  *)
 (** Write an Imp program that sums the numbers from [1] to
@@ -1375,15 +1375,32 @@ Proof.
    Prove that this program executes as intended for [X] = [2]
    (this is trickier than you might expect). *)
 
-Definition pup_to_n : com
-  (* REPLACE THIS LINE WITH ":= _your_definition_ ." *). Admitted.
+Definition pup_to_n : com :=
+  Y ::= 0;;
+  WHILE ! (X = 0) DO
+    Y ::= Y + X;;
+    X ::= X - 1
+  END.
 
 Theorem pup_to_2_ceval :
   pup_to_n / { X --> 2 }
      \\ { X --> 2 ; Y --> 0 ; Y --> 2 ; X --> 1 ; Y --> 3 ; X --> 0 }.
 Proof.
-  (* FILL IN HERE *) Admitted.
-(** [] *)
+  unfold pup_to_n.
+  apply E_Seq with { X --> 2; Y --> 0}. 
+  - apply E_Ass. reflexivity.
+  - apply E_WhileTrue with { X --> 2; Y --> 0; Y --> 2; X --> 1}. 
+    + reflexivity.
+    + apply E_Seq with { X --> 2; Y --> 0; Y --> 2}. 
+      * apply E_Ass. reflexivity.
+      * apply E_Ass. reflexivity.
+    + apply E_WhileTrue with { X --> 2; Y --> 0; Y --> 2; X --> 1; Y --> 3; X --> 0}. 
+      * reflexivity.
+      * apply E_Seq with { X --> 2; Y --> 0; Y --> 2; X --> 1; Y --> 3}. 
+      { apply E_Ass. reflexivity. }
+      { apply E_Ass. reflexivity. }
+      * apply E_WhileFalse. reflexivity.
+Qed. 
 
 (* ================================================================= *)
 (** ** Determinism of Evaluation *)
